src/ConcurrentSemantics.v
@@ -1,0 +1,190 @@
+(* This part of the work is based on https://dl.acm.org/doi/10.1145/3123569.3123576 *)
+Require Export SubstSemantics.
+
+Import ListNotations.
+
+Definition Mailbox : Set := list Exp.
+Definition Process : Set := FrameStack * Exp * Mailbox.
+
+Inductive Action : Set :=
+| ASend (p : PID) (t : Exp)
+| AReceive (t : Exp)
+| AArrive (t : Exp)
+| AInternal.
+
+Fixpoint find_clause (v : Exp) (c : list (Pat * Exp)) : option (Exp * list Exp) :=
+match c with
+| [] => None
+| (p, e)::xs => match match_pattern p v with
+                | None => find_clause v xs
+                | Some l => Some (e, l)
+                end
+end.
+
+Fixpoint receive (m : Mailbox) (c : list (Pat * Exp)) : option (Exp * Exp * list Exp) :=
+match m with
+| [] => None
+| m::ms => match find_clause m c with
+           | Some (e, l) => Some (m, e, l)
+           | None => receive ms c
+           end
+end.
+
+Definition pop (v : Exp) (m : Mailbox) := remove Exp_eq_dec v m.
+
+Reserved Notation "p -⌈ a ⌉-> p'" (at level 50).
+Inductive processLocalSemantics : Process -> Action -> Process -> Prop :=
+| p_local fs e fs' e' mb :
+  ⟨fs, e⟩ --> ⟨fs', e'⟩
+->
+  (fs, e, mb) -⌈ AInternal ⌉-> (fs', e', mb)
+
+| p_send_local fs e ι mb :
+  (fs, ESend ι e, mb) -⌈ AInternal ⌉-> (FSend ι :: fs, e, mb)
+
+| p_arrive mb mb' fs e v : VALCLOSED v -> mb' = mb ++ [v] ->
+  (fs, e, mb) -⌈ AArrive v ⌉-> (fs, e, mb')
+
+| p_send ι v mb fs :
+  (FSend ι :: fs, v, mb) -⌈ ASend ι v ⌉-> (fs, v, mb)
+
+| p_receive mb l fs e m mb' bindings :
+  receive mb l = Some (m, e, bindings) -> mb' = pop m mb
+->
+  (fs, EReceive l, mb) -⌈ AReceive m ⌉-> (fs, e.[list_subst bindings idsubst], mb')
+
+where "p -⌈ a ⌉-> p'" := (processLocalSemantics p a p').
+
+Inductive LabelStar {A B : Type} (r : A -> B -> A -> Prop) : A -> nat -> list B -> A -> Prop :=
+| lsrefl x : LabelStar r x 0 [] x
+| lsstep x l ls y z k : r x l y -> LabelStar r y k ls z -> LabelStar r x (S k) (l::ls) z.
+
+Notation "x -⌈ k | xs ⌉-> y" := (LabelStar processLocalSemantics x k xs y) (at level 50).
+
+(******************************************************************************)
+(****************************   NODES  ****************************************)
+(******************************************************************************)
+
+Require Import Coq.FSets.FMapList.
+Require Import Coq.Structures.OrderedTypeEx.
+
+Module Import NatMap := FMapList.Make(Nat_as_OT).
+
+Definition Node := t Process.
+Definition par (pid : PID) (proc: Process) (n : Node) : Node := add pid proc n.
+
+Notation "pid : p ||| n" := (par pid p n) (at level 30, right associativity).
+
+Reserved Notation "n -[ a | ι ]ₙ-> n'" (at level 50).
+Inductive nodeSemantics : Node -> Action -> PID -> Node -> Prop :=
+| nsend1 p p' q q' Π Π' ι ι' t :
+  find ι Π = Some p -> find ι' Π = Some q ->
+  Π' = ι : p' ||| ι' : q' ||| Π ->
+  p -⌈ASend ι' t⌉-> p' -> q -⌈AArrive t⌉-> q' -> ι <> ι'
+->
+  Π -[ASend ι' t | ι]ₙ-> Π'
+
+| nsend2 p p' p'' t ι Π Π' :
+  find ι Π = Some p -> Π' = ι : p'' ||| Π ->
+  p -⌈ASend ι t⌉-> p' -> p' -⌈AArrive t⌉-> p'' (** two transitions, because this is atomic! *)
+->
+  Π -[ASend ι t | ι]ₙ-> Π'
+
+| nsend3 p p' ι ι' Π Π' t :
+  find ι Π = Some p -> find ι' Π = None ->
+  Π' = ι : p' ||| Π ->
+  p -⌈ASend ι' t⌉-> p'
+->
+  Π -[ASend ι' t | ι]ₙ-> Π'
+
+| nreceive p p' t Π Π' ι :
+  find ι Π = Some p -> Π' = ι : p' ||| Π ->
+  p -⌈AReceive t⌉-> p'
+->
+  Π -[AReceive t | ι]ₙ-> Π'
+
+| ninternal p p' Π Π' ι :
+  find ι Π = Some p -> Π' = ι : p' ||| Π ->
+  p -⌈AInternal⌉-> p'
+->
+  Π -[AInternal | ι]ₙ-> Π'
+
+where "n -[ a | ι ]ₙ-> n'" := (nodeSemantics n a ι n').
+
+Reserved Notation "n -[ k | l ]ₙ->* n'" (at level 50).
+Inductive closureNodeSem : Node -> nat -> list (Action * PID) -> Node -> Prop :=
+| nrefl n : n -[ 0 | [] ]ₙ->* n
+| ntrans n n' n'' k l a ι:
+  n -[a|ι]ₙ-> n' -> n' -[k|l]ₙ->* n''
+->
+  n -[S k | (a,ι)::l]ₙ->* n''
+where "n -[ k | l ]ₙ->* n'" := (closureNodeSem n k l n').
+
+Definition nullnode : Node := empty Process.
+
+(*
+  0 -[ 1 + 1 ]-> 1
+  1 -[ 2 ]-> 3
+  2 -[ 3 ]-> 3
+  3 : 2 + 3 == 5
+*)
+Goal exists acts k,
+  0 : ([], ESend 1 (EPlus (ELit 1) (ELit 1)), []) |||
+  1 : ([], EReceive [(PVar, ESend 3 (EVar 0))], []) |||
+  2 : ([], ESend 3 (ELit 3), []) |||
+  3 : ([], EReceive [(PVar, EReceive [(PVar, EPlus (EVar 0) (EVar 1))])], []) ||| nullnode
+  -[ k | acts ]ₙ->*
+  0 : ([], ELit 2, []) |||
+  1 : ([], ELit 2, []) |||
+  2 : ([], ELit 3, []) |||
+  3 : ([], ELit 5, []) ||| nullnode.
+Proof.
+  eexists. exists 15.
+  (* Some steps with 0 *)
+  eapply ntrans. eapply ninternal with (ι := 0); cbn; try reflexivity.
+  apply p_send_local.
+  eapply ntrans. eapply ninternal with (ι := 0); cbn; try reflexivity.
+  constructor. constructor.
+  eapply ntrans. eapply ninternal with (ι := 0); cbn; try reflexivity.
+  constructor. constructor. constructor.
+
+  (* Some steps with 2 *)
+  eapply ntrans. eapply ninternal with (ι := 2); cbn; try reflexivity.
+  apply p_send_local.
+  eapply ntrans. eapply nsend1 with (ι := 2) (ι' := 3); cbn; try reflexivity.
+  constructor.
+  constructor. constructor. simpl. reflexivity. lia.
+
+  (* Again with 0 *)
+  eapply ntrans. eapply ninternal with (ι := 0); cbn; try reflexivity.
+  constructor. constructor.
+  eapply ntrans. eapply nsend1 with (ι := 0) (ι' := 1); cbn; try reflexivity.
+  constructor. constructor. constructor. reflexivity. lia.
+  (* Now with 1 *)
+  eapply ntrans. eapply nreceive with (ι := 1); cbn; try reflexivity.
+  constructor; try reflexivity.
+  eapply ntrans. eapply ninternal with (ι := 1); cbn; try reflexivity.
+  apply p_send_local.
+  eapply ntrans. eapply nsend1 with (ι := 1) (ι' := 3); cbn; try reflexivity.
+  constructor. constructor. constructor. reflexivity. lia.
+  (* Mailbox processing for 3 *)
+  eapply ntrans. eapply nreceive with (ι := 3); cbn; try reflexivity.
+  constructor; try reflexivity. cbn.
+  break_match_goal. 2: congruence.
+  break_match_goal. congruence.
+  eapply ntrans. eapply nreceive with (ι := 3); cbn; try reflexivity.
+  constructor; try reflexivity.
+  break_match_goal. 2: congruence.
+  cbn. break_match_goal. 2: congruence.
+
+  eapply ntrans. eapply ninternal with (ι := 3); cbn; try reflexivity.
+  constructor. constructor.
+  eapply ntrans. eapply ninternal with (ι := 3); cbn; try reflexivity.
+  constructor. constructor. constructor.
+  eapply ntrans. eapply ninternal with (ι := 3); cbn; try reflexivity.
+  constructor. constructor. cbn.
+  
+  unfold par, add.
+  apply nrefl.
+Qed.
+
